递归下降法
```cpp
#include <bits/stdc++.h>
using namespace std;
int expression();
int term();
int factor();
int main(){
    cout<<expression();
    return 0;
}
int expression(){
    int result=term();
    while(1){
        char c=cin.peek();
        if(c=='+'||c=='-'){
            cin.get();
            if(c=='+'){
                result+=term();
            }else{
                result-=term();
            }
        }else break;
    }
    return result;
}
int term(){
    int result=factor();
    while(1){
        char c=cin.peek();
        if(c=='*'||c=='/'){
            cin.get();
            if(c=='*'){
                result*=factor();
            }else{
                result/=factor();
            }
        }else break;
    }
    return result;
}
int factor(){
    int result=0;
    char c=cin.peek();
    if(c=='('){
       cin.get();
       result=expression();
       cin.get();
    }else{
        while(isdigit(c)){
            cin.get();
            result=result*10+c-'0';
            c=cin.peek();
        }
    }
    return result;
}
```
